Trusted mem read: finish sensor enclave proof

theories/examples/enclaves/trusted_memory_readout_code.v
@@ -13,8 +13,42 @@ Class ClientSensor := {
     sensor_mmio_addr  : Addr;
   }.
 
+Section SensorEnclaveData.
+
+  Definition one_shotR : cmra := authR (optionUR unitO).
+  Class one_shotG Σ := { #[local] one_shot_inG :: inG Σ one_shotR }.
+
+  Definition one_shotΣ : gFunctors := #[GFunctor one_shotR].
+  #[export] Instance subG_one_shotΣ {Σ} : subG one_shotΣ Σ → one_shotG Σ.
+  Proof. solve_inG. Qed.
+
+  Context {Σ:gFunctors} {oneshotg : one_shotG Σ}.
+
+  Definition pending_auth (γ : gname) : iProp Σ :=
+    own γ (● None).
+  Definition shot_auth (γ : gname) : iProp Σ :=
+    own γ (● Some ()).
+  Definition shot_token (γ : gname) : iProp Σ :=
+    own γ (◯ Some ()).
+
+  Lemma pending_alloc :
+    ⊢ |==> ∃ γ, pending_auth γ.
+  Proof. iApply own_alloc. by apply auth_auth_valid. Qed.
+
+
+  Lemma shoot (γ : gname) :
+    pending_auth γ ==∗ shot_auth γ ∗ shot_token γ.
+  Proof.
+    iIntros "H". rewrite -own_op.
+    iApply (own_update with "H").
+    by apply auth_update_alloc, alloc_option_local_update.
+  Qed.
+
+End SensorEnclaveData.
+
 Section trusted_memory_readout_example.
   Context {Σ:gFunctors} {ceriseg:ceriseG Σ} {sealsg : sealStoreG Σ}
+    {oneshotg : one_shotG Σ}
     `{reservedaddresses : ReservedAddresses}
     {nainv: logrel_na_invs Σ} `{MP: MachineParameters}.
   Context {CS: ClientSensor}.
@@ -45,8 +79,8 @@ Section trusted_memory_readout_example.
      - r_t0 = return pointer
      - r_t1 = mmio addr capability
      Returns:
-     - public signing key:      r_t1 = (U, σ__a+1, σ__a+2, σ__a+1)
-     - read_sensor entry point: r_t2 = (E, sensor, sensor_end, sensor_read)
+     - public signing key:      r_t1 = (U, σ__s+1, σ__s+2, σ__s+1)
+     - read_sensor entry point: r_t2 = Sealed σ__s+1 (E, sensor, sensor_end, sensor_read)
    *)
   Definition sensor_instrs_init (begin init read fail : Z) : list instr :=
     let RW := encodePerm RW in
@@ -88,21 +122,21 @@ Section trusted_memory_readout_example.
 
       (* Get the seal/unseal master capability and switch to signing.  *)
       Lea r_t3 (-1)%Z;         (* r_t3 = (RW, data, data_end, data) *)
-      Load r_t1 r_t3;          (* r_t1 = (SU, σ__a, σ__a+2, σ__a) *)
-      Lea r_t1 1%Z;            (* r_t1 = (SU, σ__a, σ__a+2, σ__a+1) *)
+      Load r_t1 r_t3;          (* r_t1 = (SU, σ__s, σ__s+2, σ__s) *)
+      Lea r_t1 1%Z;            (* r_t1 = (SU, σ__s, σ__s+2, σ__s+1) *)
 
       (* Construct read_sensor entry point. *)
       Lea r_t2 (read - begin); (* r_t2 = (RX, sensor, sensor_end, sensor_read) *)
       Restrict r_t2 E;         (* r_t2 = (E, sensor, sensor_end, sensor_read) *)
 
       (* Sign the entry point capability. *)
-      Seal r_t2 r_t1 r_t2 ;    (* r_t2 = Sealed σ__a+1 (E, sensor, sensor_end, sensor_read) *)
+      Seal r_t2 r_t1 r_t2 ;    (* r_t2 = Sealed σ__s+1 (E, sensor, sensor_end, sensor_read) *)
 
       (* Create signing public key *)
-      GetA r_t3 r_t1;          (* r_t3 = σ__a+1 *)
-      GetE r_t4 r_t1;          (* r_t4 = σ__a+2 *)
-      Subseg r_t1 r_t3 r_t4;   (* r_t1 = (SU, σ__a+1, σ__a+2, σ__a+1) *)
-      Restrict r_t1 U;         (* r_t1 = (U, σ__a+1, σ__a+2, σ__a+1) *)
+      GetA r_t3 r_t1;          (* r_t3 = σ__s+1 *)
+      GetE r_t4 r_t1;          (* r_t4 = σ__s+2 *)
+      Subseg r_t1 r_t3 r_t4;   (* r_t1 = (SU, σ__s+1, σ__s+2, σ__s+1) *)
+      Restrict r_t1 U;         (* r_t1 = (U, σ__s+1, σ__s+2, σ__s+1) *)
 
       (* Jump back to adversary. *)
       Jmp r_t0
@@ -121,10 +155,8 @@ Section trusted_memory_readout_example.
      - r_t0 return pointer
      - r_t1 sensor addr (mmio_a)
      - r_t2 return value (= 42)
-     Clobbers: r_t3
-   *)
+     Clobbers: r_t3 *)
   Definition sensor_instrs_read (begin read : Z) : list instr :=
-    let ROperm := encodePerm RO in
     [ Mov r_t1 PC;                    (* r_t1 = (RX, sensor, sensor_end, sensor_read) *)
       Lea r_t1 (begin - read);        (* r_t1 = (RX, sensor, sensor_end, sensor) *)
       Load r_t1 r_t1;                 (* r_t1 = (RW, data_b, data_e, ?a) *)
@@ -138,7 +170,7 @@ Section trusted_memory_readout_example.
       Lea r_t1 1;                     (* r_t1 = (RW, data_b, data_e, data_b+1) *)
       Load r_t1 r_t1;                 (* r_t1 = (RW, mmio_b, mmio_e, mmio_a) *)
       Load r_t2 r_t1;                 (* r_t2 = sensor value (42) *)
-      GetA r_t1 r_t1;                 (* r_t1 = mmio_a *)
+      GetA r_t1 r_t1;                 (* r_t3 = mmio_a *)
 
       (* Return to caller *)
       Jmp r_t0
@@ -149,25 +181,25 @@ Section trusted_memory_readout_example.
   Definition sensor_prelcode_read (init read : Z): list LWord :=
     encodeInstrsLW (sensor_instrs_read init read).
 
-  Definition sensor_init_off : Z := 1.
+  Definition sensor_init_off : Z := 0.
   Definition sensor_init_len : nat :=
     Eval cbv in length (sensor_instrs_init 0 0 0 0).
   Definition sensor_read_off : Z :=
-    Eval cbv in sensor_init_off + length (sensor_instrs_init 0 0 0 0).
+    Eval cbv in length (sensor_instrs_init 0 0 0 0).
   Definition sensor_read_len : nat :=
     Eval cbv in length (sensor_instrs_read 0 0).
   Definition sensor_fail_off : Z :=
     Eval cbv in sensor_read_off + sensor_read_len.
 
   Definition sensor_code_init : list Word :=
-    sensor_precode_init 0 sensor_init_off sensor_read_off sensor_fail_off.
+    sensor_precode_init (-1)%Z sensor_init_off sensor_read_off sensor_fail_off.
   Definition sensor_lcode_init : list LWord :=
-    sensor_prelcode_init 0 sensor_init_off sensor_read_off sensor_fail_off.
+    sensor_prelcode_init (-1)%Z sensor_init_off sensor_read_off sensor_fail_off.
 
   Definition sensor_code_read : list Word :=
-    sensor_precode_read 0 sensor_read_off.
+    sensor_precode_read (-1)%Z sensor_read_off.
   Definition sensor_lcode_read : list LWord :=
-    sensor_prelcode_read 0 sensor_read_off.
+    sensor_prelcode_read (-1)%Z sensor_read_off.
 
   Definition sensor_code : list Word :=
        sensor_code_init
@@ -188,27 +220,33 @@ Section trusted_memory_readout_example.
 
   Program Definition f42 : Addr := (finz.FinZ 42 eq_refl eq_refl).
 
-  (* The contract that the read sensor entry point should satisfy.  *)
-  Definition sensor_enclave_read_sensor_contract
-    (code_b code_e code_a : Addr) (code_v : Version) (ret : LWord) (φ : val → iPropI Σ) : iProp Σ :=
-    □ (   na_own logrel_nais ⊤
-        ∗ PC ↦ᵣ LCap E code_b code_e code_a code_v
-        ∗ r_t0 ↦ᵣ ret
-        ∗ (∃ w1, r_t1 ↦ᵣ w1)
-        ∗ (∃ w2, r_t2 ↦ᵣ w2)
-        ∗ (∃ w3, r_t3 ↦ᵣ w3)
-        ∗ ▷ (  na_own logrel_nais ⊤
-               ∗ PC ↦ᵣ updatePcPermL ret
-               ∗ (∃ b e v, r_t0 ↦ᵣ LCap O b e f42 v
-               ∗ (∃ w1, r_t1 ↦ᵣ w1)
-               ∗ (∃ w2, r_t2 ↦ᵣ w2)
-               ∗ (∃ w3, r_t3 ↦ᵣ w3)
-                 -∗ WP Seq (Instr Executable) {{ φ }}))
-          -∗ WP Seq (Instr Executable) {{ φ }}).
+  Definition sensor_one_shot_inv (γ : gname) data_b data_e data_v : iProp Σ :=
+    (pending_auth γ ∗ (∃ enclave_data, [[(data_b ^+ 1)%a,data_e]]↦ₐ{data_v}[[enclave_data]]) ∨
+     shot_token γ ∗
+       (⌜ withinBounds data_b data_e (data_b ^+ 1)%a = true ⌝ ∧
+        ∃ mmio_b mmio_e mmio_a mmio_v,
+           ((data_b ^+ 1)%a, data_v) ↦ₐ LCap RW mmio_b mmio_e mmio_a mmio_v
+         ∗ ⌜ withinBounds mmio_b mmio_e mmio_a = true ⌝
+         ∗ (mmio_a, mmio_v) ↦ₐ LInt 42)).
+
+  Definition sensor_na_inv pc_v data_b data_e data_a data_v ot γ : iProp Σ :=
+    let pc_b := sensor_begin_addr in
+    let cf_b := (pc_b ^+ 1)%a in
+    (codefrag cf_b pc_v sensor_lcode
+     ∗ (pc_b, pc_v) ↦ₐ LCap RW data_b data_e data_a data_v
+     ∗ (data_b, data_v) ↦ₐ LSealRange (true, true) ot (ot ^+ 2)%f ot
+     ∗ (sensor_one_shot_inv γ data_b data_e data_v)).
 
   (* The sensor enclave only signs the sentry to the read_sensor entry point. *)
   Definition sealed_sensor (w : LWord) : iProp Σ :=
-    (∃ b e a v, ⌜ w = LCap E b e a v ⌝ ∧ ∀ ret φ, sensor_enclave_read_sensor_contract b e a v ret φ).
+    let pc_b := sensor_begin_addr in
+    let pc_e := (pc_b ^+ (sensor_code_len + 1))%a in
+    let cf_b := (pc_b ^+ 1)%a in
+    (∃ pc_v data_b data_e data_a data_v ot γ,
+          ⌜ w = LCap E pc_b pc_e (cf_b ^+ sensor_read_off)%a pc_v ⌝
+        ∗ shot_token γ
+        ∗ na_inv logrel_nais (system_invN.@hash_sensor)
+            (sensor_na_inv pc_v data_b data_e data_a data_v ot γ)).
 
   Definition sealed_sensor_ne : (leibnizO LWord) -n> (iPropO Σ) :=
     λne (w : leibnizO LWord), sealed_sensor w%I.
@@ -218,13 +256,6 @@ Section trusted_memory_readout_example.
 
   Definition seal_pred_sensor (τ : OType) := seal_pred τ sealed_sensor.
   Definition valid_sealed_sensor_cap (w : LWord) (τ : OType) := valid_sealed w τ sealed_sensor.
-  Lemma sealed_sensor_interp (lw : LWord) : sealed_sensor lw -∗ fixpoint interp1 lw.
-  Proof.
-    iIntros "(%b & %e & %a & %v & -> & Hsealed)".
-    rewrite fixpoint_interp1_eq /=.
-    iIntros (lregs) "!> !> ([%Hfullmap #Hinterp_map] & Hrmap & Hna)".
-    admit.
-  Admitted.
 
   (* Trusted Compute Custom Predicates *)
   Definition sensor_enclave_pred : CustomEnclave :=
@@ -259,127 +290,230 @@ Section trusted_memory_readout_example.
   (* Expect:
      - PC := (RX, client, client_end, client_init)
      - r_t0 return pointer
-     - r_t1 read_sensor entry point (E, sensor, sensor_end, sensor_read)
-     - r_t2 sensor public signing key     (U, σ__s, σ__s+1, σ__s)
-     - r_t3 sensor public encryption key  (S, σ__s+1, σ__s+2, σ__s+1)
+     - r_t1 sensor public signing key (U, σ__s+1, σ__s+2, σ__s+1)
+     - r_t2 sensor read entry point (Sealed σ__s+1 (E, sensor, sensor_end, sensor_read))
      Returns:
-     - r_t1 client_use_sensor entry point (E, client, client_end, client_use_sensor)
-     - r_t2 client public signing key:    (U, σ__c, σ__c+1, σ__c)
-     - r_t3 client public encryption key: (S, σ__c+1, σ__c+2, σ__c+1)
+     - r_t0 return pointer
+     - r_t1 client_use_sensor entry point Sealed σ__c+1 (E, client, client_end, client_use_sensor)
+     - r_t2 client public signing key:    (U, σ__c+1, σ__c+2, σ__c+1)
    *)
-  Definition client_enclave_code_init_instrs
-    (client_init client_use client_fail : Z)
-    (hash_sensor : Z)
-    : list instr :=
-    let Eperm := encodePerm E in
-    let Sperm := encodeSealPerms (true, false) in
-    let Uperm := encodeSealPerms (false, true) in
-    [
+  Definition client_instrs_init (begin init use fail : Z) : list instr :=
+    let E := encodePerm E in
+    let U := encodeSealPerms (false, true) in
+    [ Mov r_t3 PC;             (* r_t3 = (RX, client, client_end, client_init) *)
 
-        (* Get and keep a pointer to a fail instruction. *)
-        Mov r_t4 PC;
-        Lea r_t4 (client_fail - client_init);
+      (* Get and keep a pointer to a fail instruction. *)
+      Lea r_t3 (fail - init);  (* r_t3 = (RX, client, client_end, client_fail) *)
 
-        (* Attest the sensor enclave's signing key. *)
-        GetA r_t5 r_t2;             (* r_t5 := ?σ__s *)
-        EStoreId r_t5 r_t5;         (* r_t5 := ?hash_sensor *)
-        (* Ensure the identity *)
-        Sub r_t5 r_t5 hash_sensor;
-        Jnz r_t4 r_t5;
+      (* Unseal the read entry point capabilitiy. *)
+      UnSeal r_t2 r_t1 r_t2;   (* r_t2 = ?(E, sensor, sensor_end, sensor_read) *)
 
-        (* Attest the sensor enclave's encryption key. *)
-        GetA r_t5 r_t3;             (* r_t5 := ?σ__s+1 *)
-        EStoreId r_t5 r_t5;         (* r_t5 := ?hash_sensor *)
-        (* Ensure the identity *)
-        Sub r_t5 r_t5 hash_sensor;
-        Jnz r_t4 r_t5;
+      (* Attest the sensor enclave's read entry point. *)
+      GetA r_t4 r_t1;          (* r_t4 = ?σ__s *)
+      EStoreId r_t1 r_t4;      (* r_t1 = ?hash_sensor *)
+      Sub r_t1 r_t1 hash_sensor;
+      Jnz r_t3 r_t1;
 
-        (* Load the data capability. *)
-        Lea r_t4 ((client_init - 1) - client_fail);
-        Load r_t5 r_t4;             (* r_t4 = cap_data *)
+      (* Get the data capability *)
+      Lea r_t3 (begin - fail); (* r_t3 = (RX, client, client_end, client) *)
+      Load r_t1 r_t3;          (* r_t1 = (RW, data, data_end, addr) *)
+      GetB r_t4 r_t1;          (* r_t4 = data *)
+      GetA r_t5 r_t1;          (* r_t5 = addr *)
+      Sub r_t4 r_t4 r_t5;      (* r_t4 = data - addr *)
+      Lea r_t1 r_t4;           (* r_t1 = (RW, data, data_end, data) *)
 
-        (* The data capability comes from the adv which controls the cursor.
-           Move it to the beginning. *)
-        GetB r_t6 r_t5;             (* r_t6 = base (b') of cap_data *)
-        GetA r_t7 r_t5;             (* r_t7 = addr (a') of cap_data *)
-        Sub r_t6 r_t6 r_t7;         (* r_t6 = base - addr *)
-        Lea r_t5 r_t6;              (* r_t5 = cap_data with address pointing to the beginning *)
+      (* Store read sensor capability in private data. *)
+      Lea r_t1 1;              (* r_t1 = (RW, data, data_end, data+1) *)
+      Store r_t1 r_t2;
 
-        Mov r_t6 r_t5;
-        (* Store the sensor enclave's entry point.  *)
-        Lea r_t6 1;
-        Store r_t6 r_t1;
-        (* Store the sensor enclave's public signing key *)
-        Lea r_t6 1;
-        Store r_t6 r_t2;
-        (* Store the sensor enclave's public encryption key *)
-        Lea r_t6 1;
-        Store r_t6 r_t3;
-        Mov r_t6 0;
+      (* Get the seal/unseal master capability and switch to signing.  *)
+      Lea r_t1 (-1)%Z;         (* r_t1 = (RW, data, data_end, data) *)
+      Load r_t2 r_t1;          (* r_t2 = (SU, σ__c, σ__c+2, σ__c) *)
+      Lea r_t2 1%Z;            (* r_t2 = (SU, σ__c, σ__c+2, σ__c+1) *)
 
-        (* Get the use_sensor entry point. *)
-        Mov r_t1 r_t4;
-        Lea r_t1 (client_use - (client_init - 1));
-        Restrict r_t1 Eperm;    (* r_t1 = (E, client, client_end, client_use) *)
+      (* Construct read_sensor entry point. *)
+      Lea r_t3 (use - begin);  (* r_t3 = (RX, client, client_end, client_use) *)
+      Restrict r_t3 E;         (* r_t3 = (E, client, client_end, client_use) *)
 
-        (* Get the seal/unseal capability.  *)
-        Load r_t2 r_t5;         (* r_t2 = seal / unseal capability (SU, σ__c, σ__c+2, σ__c) *)
-        Mov r_t3 r_t2;          (* r_t3 = seal / unseal capability (SU, σ__c, σ__c+2, σ__c) *)
+      (* Sign the entry point capability. *)
+      Seal r_t1 r_t2 r_t3;     (* r_t1 = Sealed σ__c+1 (E, client, client_end, client_use) *)
 
-        (* Get public signing key, which is (U, σ__c, σ__c+1, σ__c) *)
-        GetB r_t4 r_t2;         (* r_t4 = σ__c *)
-        Add r_t5 r_t4 1;        (* r_t5 = σ__c+1 *)
-        Subseg r_t2 r_t4 r_t5;  (* r_t2 = (SU, σ__c, σ__c+1, σ__c) *)
-        Restrict r_t2 Uperm;    (* r_t2 = (U, σ__c, σ__c+1, σ__c) *)
+      (* Create signing public key *)
+      GetA r_t3 r_t1;          (* r_t3 = σ__c+1 *)
+      GetE r_t4 r_t1;          (* r_t4 = σ__c+2 *)
+      Subseg r_t2 r_t3 r_t4;   (* r_t2 = (SU, σ__c+1, σ__c+2, σ__c+1) *)
+      Restrict r_t2 U;         (* r_t2 = (U, σ__c+1, σ__c+2, σ__c+1) *)
 
-        (* Get public encryption key, which is (S, σ__c+1, σ__c+2, σ__c+1) *)
-        Lea r_t3 1%Z;          (* r_t3 = (SU, σ__c+1, σ__c+2, σ__c+1) *)
-        GetE r_t4 r_t3;        (* r_t4 = σ__c+2 *)
-        Subseg r_t3 r_t5 r_t4; (* r_t3 = (SU, σ__c+1, σ__c+2, σ__c+1) *)
-        Restrict r_t3 Sperm;   (* r_t3 = (S, σ__c+1, σ__c+2, σ__c+1) *)
-
-        Jmp r_t0
-      ].
-
-  Definition client_enclave_code_init_code
-    (client_init client_use client_fail : Z)
-    (hash_sensor : Z)
-    : list Word :=
-    encodeInstrsW (client_enclave_code_init_instrs client_init client_use client_fail hash_sensor).
-
-  Definition client_enclave_code_init_lcode
-    (client_init client_use client_fail : Z)
-    (hash_sensor : Z)
-    : list LWord :=
-    encodeInstrsLW (client_enclave_code_init_instrs client_init client_use client_fail hash_sensor).
-
-  (* Expect:
-     - PC := (RX, client, client_end, client_use_sensor)
-     - r_t1 pointer to buffer (arg). encrypted with the client enclave's encryption key.
-     Returns:
-   *)
-
-  Definition client_enclave_code_use_sensor
-    (client_use client_fail : Z) : list LWord :=
-
-    encodeInstrsLW [
-        Jmp r_t0
+      Jmp r_t0
     ].
 
+  Definition client_precode_init (begin init use fail : Z): list Word :=
+    encodeInstrsW (client_instrs_init begin init use fail).
+
+  Definition client_prelcode_init (begin init use fail : Z): list LWord :=
+    encodeInstrsLW (client_instrs_init begin init use fail).
+
+  (* Expect:
+     - PC := (RX, client, client_end, client_use)
+     - r_t0 return pointer
+     Returns:
+     - r_t0 return pointer
+     - r_t1 sensor addr (mmio_a)
+     - r_t2 return value (= 84)
+     Clobbers: r_t3, r_t4 *)
+  Definition client_instrs_use (begin use : Z) : list instr :=
+    [ Mov r_t1 PC;                    (* r_t1 = (RX, client, client_end, client_use) *)
+
+      Lea r_t1 (begin - use);         (* r_t1 = (RX, client, client_end, client) *)
+      Load r_t1 r_t1;                 (* r_t1 = (RW, data_b, data_e, ?a) *)
+      GetB r_t2 r_t1;                 (* r_t2 = data_b *)
+      GetA r_t3 r_t1;                 (* r_t3 = ?a *)
+      Sub r_t2 r_t2 r_t3;             (* r_t2 = data_b - ?a *)
+      Lea r_t1 r_t2;                  (* r_t1 = (RW, data_b, data_e, data_b) *)
+
+      (* Load sensor enclave read entry point *)
+      Lea r_t1 1;                     (* r_t1 = (RW, data_b, data_e, data_b+1) *)
+      Load r_t1 r_t1;                 (* r_t1 = (E, sensor, sensor_end, sensor_read) *)
+
+      (* Save return pointer to a register unclobbered by sensor read *)
+      Mov r_t4 r_t0;                  (* r_t4 = return pointer *)
+
+      (* Setup callback and jump to read sensor entry point. *)
+      Mov r_t0 PC;
+      Lea r_t0 3;                     (* r_t0 = use callback *)
+      Jmp r_t1;
+
+      (* Use Callback
+           Expect:
+           - r_t1 sensor addr (mmio_a)
+           - r_t2 sensor read return value (= 42) *)
+
+      (* Perform computation on the sensor value *)
+      Add r_t2 r_t2 r_t2;             (* r_t2 = 84 *)
+
+      (* Return to caller *)
+      Jmp r_t0
+    ].
+
+  Definition client_precode_use (init use : Z): list Word :=
+    encodeInstrsW (client_instrs_use init use).
+  Definition client_prelcode_use (init use : Z): list LWord :=
+    encodeInstrsLW (client_instrs_use init use).
+
+  Definition client_init_off : Z := 0.
+  Definition client_init_len : nat :=
+    Eval cbv in length (client_instrs_init 0 0 0 0).
+  Definition client_use_off : Z :=
+    Eval cbv in length (client_instrs_init 0 0 0 0).
+  Definition client_use_len : nat :=
+    Eval cbv in length (client_instrs_use 0 0).
+  Definition client_fail_off : Z :=
+    Eval cbv in client_use_off + client_use_len.
+
+  Definition client_code_init : list Word :=
+    client_precode_init (-1)%Z client_init_off client_use_off client_fail_off.
+  Definition client_lcode_init : list LWord :=
+    client_prelcode_init (-1)%Z client_init_off client_use_off client_fail_off.
+
+  Definition client_code_use : list Word :=
+    client_precode_use (-1)%Z client_use_off.
+  Definition client_lcode_use : list LWord :=
+    client_prelcode_use (-1)%Z client_use_off.
+
+  Definition client_code : list Word :=
+       client_code_init
+    ++ client_code_use
+    ++ encodeInstrsW [Fail].
+
+  Definition client_lcode : list LWord :=
+       client_lcode_init
+    ++ client_lcode_use
+    ++ encodeInstrsLW [Fail].
+  Definition client_code_len : nat :=
+    Eval cbv in length client_lcode.
+
+  Definition hash_client : Z :=
+    hash_concat (hash client_begin_addr) (hash client_code).
+
+  (* Sealed predicate for client enclave *)
+
+  Program Definition f84 : Addr := (finz.FinZ 84 eq_refl eq_refl).
+
+  Definition client_one_shot_inv (γ : gname) data_b data_e data_v : iProp Σ :=
+    (pending_auth γ ∗ (∃ enclave_data, [[(data_b ^+ 1)%a,data_e]]↦ₐ{data_v}[[enclave_data]]) ∨
+     shot_token γ ∗
+       (⌜ withinBounds data_b data_e (data_b ^+ 1)%a = true ⌝ ∧
+        ∃ mmio_b mmio_e mmio_a mmio_v,
+           ((data_b ^+ 1)%a, data_v) ↦ₐ LCap RW mmio_b mmio_e mmio_a mmio_v
+         ∗ ⌜ withinBounds mmio_b mmio_e mmio_a = true ⌝
+         ∗ (mmio_a, mmio_v) ↦ₐ LInt 42)).
+
+  Definition client_na_inv pc_v data_b data_e data_a data_v ot γ : iProp Σ :=
+    let pc_b := client_begin_addr in
+    let cf_b := (pc_b ^+ 1)%a in
+    (codefrag cf_b pc_v client_lcode
+     ∗ (pc_b, pc_v) ↦ₐ LCap RW data_b data_e data_a data_v
+     ∗ (data_b, data_v) ↦ₐ LSealRange (true, true) ot (ot ^+ 2)%f ot
+     ∗ (client_one_shot_inv γ data_b data_e data_v)).
+
+  (* The client enclave only signs the sentry to the use entry point. *)
+  Definition sealed_client (w : LWord) : iProp Σ :=
+    let pc_b := client_begin_addr in
+    let pc_e := (pc_b ^+ (client_code_len + 1))%a in
+    let cf_b := (pc_b ^+ 1)%a in
+    (∃ pc_v data_b data_e data_a data_v ot γ,
+          ⌜ w = LCap E pc_b pc_e (cf_b ^+ client_use_off)%a pc_v ⌝
+        ∗ shot_token γ
+        ∗ na_inv logrel_nais (system_invN.@hash_client)
+            (client_na_inv pc_v data_b data_e data_a data_v ot γ)).
+
+  Definition sealed_client_ne : (leibnizO LWord) -n> (iPropO Σ) :=
+    λne (w : leibnizO LWord), sealed_client w%I.
+
+  #[export] Instance sealed_client_persistent (w : LWord) : Persistent (sealed_client w).
+  Proof. repeat (apply bi.exist_persistent; intros). apply _. Qed.
+
+  Definition seal_pred_client (τ : OType) := seal_pred τ sealed_client.
+  Definition valid_sealed_client_cap (w : LWord) (τ : OType) := valid_sealed w τ sealed_client.
+
+  (* Trusted Compute Custom Predicates *)
+  Definition client_enclave_pred : CustomEnclave :=
+    @MkCustomEnclave Σ
+      client_code
+      client_begin_addr
+      (λ w, False%I)
+      sealed_client.
+
+  (* ------------------------ *)
+  (* ---   ENCLAVES MAP   --- *)
+  (* ------------------------ *)
+
   Definition ts_enclaves_map : custom_enclaves_map (Σ := Σ) :=
-    {[ hash_sensor := sensor_enclave_pred ]}.
+    {[ hash_sensor := sensor_enclave_pred;
+       hash_client := client_enclave_pred
+    ]}.
 
   Lemma wf_ts_enclaves_map :
     custom_enclaves_map_wf ts_enclaves_map.
   Proof.
     rewrite /custom_enclaves_map_wf /ts_enclaves_map.
     split.
-    + by rewrite map_Forall_singleton /hash_sensor /=.
-    + rewrite map_Forall_singleton.
-      apply Forall_forall. cbn.
-      intros w Hw.
-      repeat (rewrite elem_of_cons in Hw ; destruct Hw as [-> | Hw]; first done).
-      by rewrite elem_of_nil in Hw.
+    - apply (map_Forall_insert_2 (λ (I : Z) (ce : CustomEnclave), _)).
+      + by rewrite /hash_sensor /=.
+      + by rewrite map_Forall_singleton /hash_client /=.
+    - apply (map_Forall_insert_2 (λ (I : Z) (ce : CustomEnclave), _)).
+      + cbn.
+        rewrite /encodeInstrW.
+        apply Forall_forall.
+        intros w Hw.
+        repeat (rewrite elem_of_cons in Hw ; destruct Hw as [-> | Hw]; first done).
+        by rewrite elem_of_nil in Hw.
+      + rewrite map_Forall_singleton; cbn.
+        rewrite /encodeInstrW.
+        apply Forall_forall.
+        intros w Hw.
+        repeat (rewrite elem_of_cons in Hw ; destruct Hw as [-> | Hw]; first done).
+        by rewrite elem_of_nil in Hw.
   Qed.
 
   #[export] Instance contract_tsenclaves_map : CustomEnclavesMap :=
