theories/examples/enclaves/trusted_memory_readout_sensor_spec.v
@@ -4,40 +4,6 @@ From cap_machine Require Import rules logrel fundamental.
 From cap_machine Require Import proofmode.
 From cap_machine Require Import trusted_memory_readout_code.
 
-Section SensorEnclaveData.
-
-  Definition one_shotR : cmra := authR (optionUR unitO).
-  Class one_shotG Σ := { #[local] one_shot_inG :: inG Σ one_shotR }.
-
-  Definition one_shotΣ : gFunctors := #[GFunctor one_shotR].
-  #[export] Instance subG_one_shotΣ {Σ} : subG one_shotΣ Σ → one_shotG Σ.
-  Proof. solve_inG. Qed.
-
-  Context {Σ:gFunctors} {oneshotg : one_shotG Σ}.
-
-  Definition pending_auth (γ : gname) : iProp Σ :=
-    own γ (● None).
-  Definition shot_auth (γ : gname) : iProp Σ :=
-    own γ (● Some ()).
-  Definition shot_token (γ : gname) : iProp Σ :=
-    own γ (◯ Some ()).
-
-  Lemma pending_alloc :
-    ⊢ |==> ∃ γ, pending_auth γ.
-  Proof. iApply own_alloc. by apply auth_auth_valid. Qed.
-
-  Lemma shoot (γ : gname) :
-    pending_auth γ ==∗ shot_auth γ ∗ shot_token γ.
-  Proof.
-    iIntros "H". rewrite -own_op.
-    iApply (own_update with "H").
-    by apply auth_update_alloc, alloc_option_local_update.
-  Qed.
-
-  (* Definition sensor_dataN := nroot .@ "sensor" .@ "data". *)
-
-End SensorEnclaveData.
-
 Section SensorEnclaveProofs.
   Context {Σ:gFunctors} {ceriseg:ceriseG Σ} {sealsg: sealStoreG Σ}
     {nainv: logrel_na_invs Σ} {oneshotg : one_shotG Σ}
@@ -45,68 +11,256 @@ Section SensorEnclaveProofs.
     `{MP: MachineParameters}.
   Context {CS: ClientSensor}.
 
-  Definition one_shot_inv (γ : gname) data_b data_e data_v : iProp Σ :=
-    (pending_auth γ ∗ (∃ enclave_data, [[(data_b ^+ 1)%a,data_e]]↦ₐ{data_v}[[enclave_data]]) ∨
-     shot_token γ ∗ (∃ mmio_b mmio_e mmio_a mmio_v,
-       ((data_b ^+ 1)%a, data_v) ↦ₐ LCap RW mmio_b mmio_e mmio_a mmio_v))%I.
-
-  Lemma one_shot_update γ data_b data_e data_v (Hdatarange : (data_b < data_e)%a) :
-    one_shot_inv γ data_b data_e data_v ==∗ shot_token γ ∗
-    (⌜ (data_b ^+ 1)%a = data_e ⌝ ∨
-     (∃ lw, ((data_b ^+ 1)%a, data_v) ↦ₐ lw))%I.
+  Lemma sensor_one_shot_update γ data_b data_e data_v (Hdatarange : (data_b < data_e)%a) :
+    sensor_one_shot_inv γ data_b data_e data_v ==∗ shot_token γ ∗
+    (⌜ withinBounds data_b data_e (data_b ^+ 1)%a = false ⌝ ∨
+     (⌜ withinBounds data_b data_e (data_b ^+ 1)%a = true ⌝ ∧
+       ∃ lw, ((data_b ^+ 1)%a, data_v) ↦ₐ lw))%I.
   Proof.
-    iIntros "[(Hauth & %enclave_data & Hdata)|[Htoken Hdata]]".
-    - iMod (shoot with "Hauth") as "[_ Htoken]". iModIntro. iFrame.
+    iIntros "[(Hauth & %enclave_data & Hdata)|(Htoken & %Hdatabounds & Hdata)]".
+    - iMod (shoot with "Hauth") as "[H Htoken]". iModIntro. iFrame.
       iDestruct (big_sepL2_length with "Hdata") as "%Hdata_len".
       rewrite map_length finz_seq_between_length /finz.dist /= in Hdata_len.
       destruct enclave_data as [|lw enclave_data].
-      + iLeft. iPureIntro. solve_addr.
+      + iLeft. iPureIntro. apply andb_false_intro2. solve_addr.
       + iRight.
+        assert (data_b ^+ 2 <= data_e)%a by solve_addr.
         iDestruct (region_mapsto_cons with "Hdata") as "[Hts_mmio Hts_data]"; last iFrame.
-        { transitivity (Some (data_b ^+ 2)%a); try solve_addr. }
-        { solve_addr. }
+        { transitivity (Some (data_b ^+ 2)%a); solve_addr. }
+        { assumption. }
+        iSplit. iPureIntro. apply le_addr_withinBounds; solve_addr.
         iExists _. iFrame.
-    - iModIntro. iSplitL "Htoken". done. iRight.
-      iDestruct "Hdata" as "(%mmio_b & %mmio_e & %mmio_a & %mmio_v & H)".
+    - iModIntro. iSplitL "Htoken". done. iRight. iSplitR. done.
+      iDestruct "Hdata" as "(%mmio_b & %mmio_e & %mmio_a & %mmio_v & Hdata & H & Hmmio)".
       iExists _. done.
   Qed.
 
-  Lemma sensor_enclave_read_sensor_correct n pc_v data_b data_e data_a data_v
+  (* The contract that the read sensor entry point should satisfy.  *)
+  Definition sensor_enclave_read_sensor_contract
+    (code_b code_e code_a : Addr) (code_v : Version) (ret : LWord) (φ : val → iPropI Σ) : iProp Σ :=
+    na_own logrel_nais ⊤
+    ∗ PC ↦ᵣ LCap RX code_b code_e code_a code_v
+    ∗ r_t0 ↦ᵣ ret
+    ∗ (∃ w1, r_t1 ↦ᵣ w1)
+    ∗ (∃ w2, r_t2 ↦ᵣ w2)
+    ∗ (∃ w3, r_t3 ↦ᵣ w3)
+    ∗ ▷ (  na_own logrel_nais ⊤
+         ∗ PC ↦ᵣ updatePcPermL ret
+         ∗ (r_t0 ↦ᵣ ret)
+         ∗ (∃ mmio_a : Z, r_t1 ↦ᵣ LInt mmio_a)
+         ∗ (r_t2 ↦ᵣ LInt 42)
+         ∗ (∃ w3, r_t3 ↦ᵣ w3 ∗ interp w3)
+           -∗ WP Seq (Instr Executable) {{ φ }})
+      -∗ WP Seq (Instr Executable) {{ φ }}.
+
+  Lemma sensor_enclave_read_sensor_correct n pc_v data_b data_e data_a data_v γ
     ot ret φ :
     let pc_b := sensor_begin_addr in
-    let pc_e := (pc_b ^+ (sensor_code_len + 1))%a in
+    let pc_e := (pc_b ^+ (length sensor_lcode + 1))%a in
     let cf_b := (pc_b ^+ 1)%a in
-    let cf_e := (cf_b ^+ sensor_read_len)%a in
-    (pc_b + (sensor_code_len + 1) = Some pc_e)%a ->
-    (data_b < data_e)%a ->
+    let cf_e := (cf_b ^+ length sensor_lcode)%a in
 
-      system_inv
-    ∗ na_inv logrel_nais n
-        (codefrag cf_b pc_v sensor_lcode
-         ∗ (pc_b, pc_v) ↦ₐ LCap RW data_b data_e data_a data_v
-         ∗ (data_b, data_v) ↦ₐ LSealRange (true, true) ot (ot ^+ 2)%f ot
-         ∗ (∃ γ : gname, one_shot_inv γ data_b data_e data_v))
-    ⊢ sensor_enclave_read_sensor_contract pc_b pc_e (pc_b ^+ sensor_read_off)%a pc_v ret φ.
+      shot_token γ
+    ∗ na_inv logrel_nais n (sensor_na_inv pc_v data_b data_e data_a data_v ot γ)
+
+    ⊢ sensor_enclave_read_sensor_contract pc_b pc_e (cf_b ^+ sensor_read_off)%a pc_v ret φ.
   Proof.
-    iIntros (pc_b pc_e cf_b cf_e Hpc_b_e Hdata_b_e) "[#Henclave_inv #Hts_inv] !>".
+    iIntros (pc_b pc_e cf_b cf_e (* Hpc_b_e *) ) "#(Htoken & Hts_inv)".
     iIntros "(Hna & HPC & Hr0 & [%lw1 Hr1] & [%lw2 Hr2] & [%lw3 Hr3] & Hret)".
 
-    assert (SubBounds pc_b pc_e cf_b cf_e).
-    { subst pc_e pc_b cf_e cf_b.
-      rewrite /sensor_code_len /sensor_read_off /sensor_read_len.
-      solve_addr. }
-    assert (withinBounds pc_b pc_e pc_b = true) as Hpcbounds.
-    { subst pc_e; apply le_addr_withinBounds; solve_addr. }
-    assert (withinBounds data_b data_e data_b = true) as Hdatabounds.
-    { apply le_addr_withinBounds; solve_addr. }
-
     iMod (na_inv_acc with "Hts_inv Hna") as
-      "(>(Hts_code & Hts_keys & Hts_addr & [%γ Hts_data]) & Hna & Hclose)"; [solve_ndisj ..|].
+      "(>(Hts_code & Hts_keys & Hts_addr & Hts_data) & Hna & Hclose)"; [solve_ndisj ..|].
 
     (* Code memory *)
     codefrag_facts "Hts_code".
 
-  Admitted.
+    assert (SubBounds pc_b pc_e cf_b cf_e).
+    { subst pc_e pc_b cf_e cf_b.
+      solve_addr. }
+    assert (withinBounds pc_b pc_e pc_b = true) as Hpcbounds.
+    { subst pc_b pc_e. apply le_addr_withinBounds; solve_addr. }
+
+    (* Data memory *)
+    iDestruct ("Hts_data") as "[(Hauth & _)|(_ & %Hwb & %mmio_b & %mmio_e & %mmio_a & %mmio_v & Hts_data & %Hmmiobounds & Hts_mmio)]".
+    { iCombine "Hauth Htoken" gives % [Hl _]%auth_both_valid_discrete.
+      exfalso. clear -Hl. apply option_included in Hl.
+      destruct Hl as [|(? & ? & ? & ? & ?)]; discriminate. }
+
+
+    (* Prove the spec *)
+    iInstr "Hts_code". (* Mov r_t1 PC *)
+
+    iInstr "Hts_code". (* Lea r_t1 (begin - read) *)
+    { transitivity (Some pc_b); [|easy].
+      rewrite /sensor_read_off. subst cf_b pc_b. solve_addr. }
+
+    iInstr "Hts_code". (* Load r_t1 r_t1 *)
+    iInstr "Hts_code". (* GetB r_t2 r_t1 *)
+    iInstr "Hts_code". (* GetA r_t3 r_t1 *)
+    iInstr "Hts_code". (* Sub r_t2 r_t2 r_t3 *)
+    iInstr "Hts_code". (* Lea r_t1 r_t2 *)
+    { transitivity (Some data_b); solve_addr. }
+
+    iInstr "Hts_code". (* Lea r_t1 1 *)
+    { transitivity (Some (data_b ^+ 1)%a); solve_addr. }
+
+    iInstr "Hts_code". (* Load r_t1 r_t1 *)
+    iInstr "Hts_code". (* Load r_t2 r_t1 *)
+    auto.
+    wp_instr. iInstr_lookup "Hts_code" as "Hi" "Hts_code".
+    iApply (wp_Get_same_success with "[$HPC $Hi $Hr1]"); try solve_pure.
+    iNext. iIntros "(HPC & Hi & Hr1)".
+    wp_pure. iInstr_close "Hts_code".
+
+    iInstr "Hts_code". (* Jmp r_t0 *)
+
+    (* Close the opened invariant *)
+    iMod ("Hclose" with "[$Hna $Hts_code $Hts_addr $Hts_keys Htoken Hts_data Hts_mmio]") as "Hna".
+    iNext. iRight. iFrame "Htoken".
+    iSplit; [easy|]. do 4 iExists _. by iFrame.
+
+    iApply ("Hret" with "[$Hna $HPC $Hr0 Hr1 Hr2 Hr3]").
+    { iSplitL "Hr1". by auto.
+      iSplitL "Hr2". by auto.
+      iExists _.
+      iSplitL "Hr3". by auto.
+      iApply interp_int. }
+  Qed.
+
+  Lemma sealed_sensor_interp (lw : LWord) :
+    □ custom_enclave_contract_gen ∗ system_inv
+    ⊢ sealed_sensor lw -∗ fixpoint interp1 lw.
+  Proof.
+    rewrite /sealed_sensor.
+    iIntros "[#Henclave_contract #Henclave_inv] Hsealed".
+    iDestruct "Hsealed" as (pc_v data_b data_e data_a data_v ot γ) "(-> & #Htoken & #Hts_inv)".
+    rewrite fixpoint_interp1_eq /=.
+
+    iIntros (lregs); iNext; iModIntro.
+    iIntros "([%Hfullmap #Hinterp_map] & Hrmap & Hna)".
+    rewrite /interp_conf.
+    rewrite /registers_mapsto.
+    iExtract "Hrmap" PC as "HPC".
+
+    set (pc_b := sensor_begin_addr).
+    set (pc_e := (pc_b ^+ (sensor_code_len + 1))%a).
+    set (cf_b := (pc_b ^+ 1)%a).
+
+    (* Prepare the necessary resources *)
+    (* Registers *)
+    assert (exists w0, lregs !! r_t0 = Some w0) as Hrt0 by apply (Hfullmap r_t0).
+    destruct Hrt0 as [w0 Hr0].
+    replace (delete PC lregs)
+      with (<[r_t0:=w0]> (delete PC lregs)).
+    2: { rewrite insert_id; auto. rewrite lookup_delete_ne; auto. }
+
+    assert (exists w1, lregs !! r_t1 = Some w1) as Hrt1 by apply (Hfullmap r_t1).
+    destruct Hrt1 as [w1 Hr1].
+    replace (delete PC lregs)
+      with (<[r_t1:=w1]> (delete PC lregs)).
+    2: { rewrite insert_id; auto. rewrite lookup_delete_ne; auto. }
+
+    assert (exists w2, lregs !! r_t2 = Some w2) as Hrt2 by apply (Hfullmap r_t2).
+    destruct Hrt2 as [w2 Hr2].
+    replace (delete PC lregs)
+      with (<[r_t2:=w2]> (delete PC lregs)).
+    2: { rewrite insert_id; auto. rewrite lookup_delete_ne; auto. }
+
+    assert (exists w3, lregs !! r_t3 = Some w3) as Hrt3 by apply (Hfullmap r_t3).
+    destruct Hrt3 as [w3 Hr3].
+    replace (delete PC lregs)
+      with (<[r_t3:=w3]> (delete PC lregs)).
+    2: { rewrite insert_id; auto. rewrite lookup_delete_ne; auto. }
+
+    (* assert (exists w4, lregs !! r_t4 = Some w4) as Hrt4 by apply (Hfullmap r_t4). *)
+    (* destruct Hrt4 as [w4 Hr4]. *)
+    (* replace (delete PC lregs) *)
+    (*   with (<[r_t4:=w4]> (delete PC lregs)). *)
+    (* 2: { rewrite insert_id; auto. rewrite lookup_delete_ne; auto. } *)
+
+    (* assert (exists w5, lregs !! r_t5 = Some w5) as Hrt5 by apply (Hfullmap r_t5). *)
+    (* destruct Hrt5 as [w5 Hr5]. *)
+    (* replace (delete PC lregs) *)
+    (*   with (<[r_t5:=w5]> (delete PC lregs)). *)
+    (* 2: { rewrite insert_id; auto. rewrite lookup_delete_ne; auto. } *)
+
+    (* EXTRACT REGISTERS FROM RMAP *)
+    (* iExtractList "Hrmap" [r_t0;r_t1;r_t2;r_t3] as ["Hr0";"Hr1";"Hr2";"Hr3"]. *)
+    iDestruct (big_sepM_delete _ _ r_t0 with "Hrmap") as "[Hr0 Hrmap]".
+    { by simplify_map_eq. }
+    iDestruct (big_sepM_delete _ _ r_t1 with "Hrmap") as "[Hr1 Hrmap]".
+    { by simplify_map_eq. }
+    iDestruct (big_sepM_delete _ _ r_t2 with "Hrmap") as "[Hr2 Hrmap]".
+    { by simplify_map_eq. }
+    iDestruct (big_sepM_delete _ _ r_t3 with "Hrmap") as "[Hr3 Hrmap]".
+    { by simplify_map_eq. }
+    (* iDestruct (big_sepM_delete _ _ r_t4 with "Hrmap") as "[Hr4 Hrmap]". *)
+    (* { by simplify_map_eq. } *)
+    (* iDestruct (big_sepM_delete _ _ r_t5 with "Hrmap") as "[Hr5 Hrmap]". *)
+    (* { by simplify_map_eq. } *)
+    replace (delete r_t3 _) with
+      ( delete r_t3 (delete r_t2 (delete r_t1 (delete r_t0 (delete PC lregs))))).
+    2:{
+      rewrite delete_insert_delete; repeat rewrite (delete_insert_ne _ r_t0) //.
+      rewrite delete_insert_delete; repeat rewrite (delete_insert_ne _ r_t1) //.
+      rewrite delete_insert_delete; repeat rewrite (delete_insert_ne _ r_t2) //.
+      rewrite delete_insert_delete; repeat rewrite (delete_insert_ne _ r_t3) //.
+      (* rewrite delete_insert_delete; repeat rewrite (delete_insert_ne _ r_t4) //. *)
+      (* rewrite delete_insert_delete; repeat rewrite (delete_insert_ne _ r_t5) //. *)
+      done.
+    }
+    iAssert (interp w0) as "Hinterp_w0".
+    { iApply "Hinterp_map";eauto;done. }
+
+    iApply (sensor_enclave_read_sensor_correct with "[$Htoken $Hts_inv]").
+    iFrame "Hna HPC Hr0".
+    iSplitL "Hr1". iExists _. iExact "Hr1".
+    iSplitL "Hr2". iExists _. iExact "Hr2".
+    iSplitL "Hr3". iExists _. iExact "Hr3".
+
+    iDestruct (jmp_to_unknown with "[$Henclave_contract $Henclave_inv] [$Hinterp_w0]") as "Hjmp".
+
+    iIntros "!> (Hna & HPC & Hr0 & [%mmio_a Hr1] & Hr2 & (%w3' & Hr3 & #Hinterp_w3'))".
+
+    (* Wrap up the registers *)
+    iDestruct (big_sepM_insert _ _ r_t0 with "[$Hrmap $Hr0]") as "Hrmap".
+    { do 3 ( rewrite lookup_delete_ne //) ; by rewrite lookup_delete. }
+    do 3 (rewrite -delete_insert_ne //=); rewrite insert_delete_insert.
+    iDestruct (big_sepM_insert _ _ r_t1 with "[$Hrmap $Hr1]") as "Hrmap".
+    { do 2 ( rewrite lookup_delete_ne //) ; by rewrite lookup_delete. }
+    do 2 (rewrite -delete_insert_ne //=); rewrite insert_delete_insert.
+    iDestruct (big_sepM_insert _ _ r_t2 with "[$Hrmap $Hr2]") as "Hrmap".
+    { do 1 ( rewrite lookup_delete_ne //) ; by rewrite lookup_delete. }
+    do 1 (rewrite -delete_insert_ne //=); rewrite insert_delete_insert.
+    iDestruct (big_sepM_insert _ _ r_t3 with "[$Hrmap $Hr3]") as "Hrmap".
+    { do 0 ( rewrite lookup_delete_ne //) ; by rewrite lookup_delete. }
+    do 0 (rewrite -delete_insert_ne //=); rewrite insert_delete_insert.
+    set (rmap' := (<[r_t3:=_]> _)).
+    iAssert ([∗ map] k↦y ∈ rmap', k ↦ᵣ y ∗ interp y)%I with "[Hrmap]" as "Hrmap".
+    {
+      subst rmap'.
+      iApply (big_sepM_sep_2 with "[Hrmap]") ; first done.
+      iApply big_sepM_insert_2; first done.
+      iApply big_sepM_insert_2; first (iApply interp_int).
+      iApply big_sepM_insert_2; first (iApply interp_int).
+      iApply big_sepM_insert_2; first done.
+      iApply big_sepM_intro.
+      iIntros "!>" (r w Hrr).
+      assert (is_Some (delete PC lregs !! r)) as His_some by auto.
+      rewrite lookup_delete_is_Some in His_some.
+      destruct His_some as [Hr _].
+      rewrite lookup_delete_ne in Hrr; auto.
+      iApply ("Hinterp_map" $! r w); auto.
+    }
+    assert (dom rmap' = all_registers_s ∖ {[PC]}).
+    {
+      repeat (rewrite dom_insert_L).
+      rewrite dom_delete_L.
+      rewrite regmap_full_dom; auto.
+    }
+
+    iApply ("Hjmp" with "[]") ; eauto ; iFrame.
+  Qed.
 
   Lemma sensor_enclave_correct
     (Ep : coPset)
@@ -140,13 +294,10 @@ Section SensorEnclaveProofs.
     iMod pending_alloc as (γ) "Hauth".
 
     iMod (na_inv_alloc logrel_nais _ (system_invN.@hash_sensor)
-            (codefrag cf_b pc_v sensor_lcode
-             ∗ (pc_b, pc_v) ↦ₐ LCap RW data_b data_e data_a data_v
-             ∗ (data_b, data_v) ↦ₐ LSealRange (true, true) ot (ot ^+ 2)%f ot
-             ∗ ∃ γ, one_shot_inv γ data_b data_e data_v)%I
+            (sensor_na_inv pc_v data_b data_e data_a data_v ot γ)
            with "[$Hts_code $Hts_addr $Hts_keys Hauth Hts_data]") as "#Hts_inv".
-    { iNext. iExists γ. iLeft. iFrame "Hauth". by iExists enclave_data. }
-    clear γ enclave_data.
+    { iNext. iLeft. iFrame "Hauth". by iExists enclave_data. }
+    clear enclave_data.
 
     assert (SubBounds pc_b pc_e cf_b cf_e) by
       (subst pc_e pc_b cf_e cf_b; rewrite /sensor_code_len; solve_addr).
@@ -161,7 +312,7 @@ Section SensorEnclaveProofs.
     iIntros "([%Hfullmap #Hinterp_map] & Hrmap & Hna)".
     rewrite /interp_conf.
     iMod (na_inv_acc with "Hts_inv Hna") as
-      "(>(Hts_code & Hts_addr & Hts_keys & [%γ Hts_data]) & Hna & Hclose)";
+      "(>(Hts_code & Hts_addr & Hts_keys & Hts_data) & Hna & Hclose)";
       [solve_ndisj ..|].
     rewrite /registers_mapsto.
     iExtract "Hrmap" PC as "HPC".
@@ -309,8 +460,9 @@ Section SensorEnclaveProofs.
     (* Check that we have exclusive access to the mmio capability. *)
     (* IsUnique r_t3 r_t1 *)
     wp_instr. iInstr_lookup "Hts_code" as "Hi" "Hts_code".
+    iDestruct (readAllowed_not_reserved with "Hinterp_w1") as "%Hnotreserved".
+    { done. }
     iApply (wp_isunique_success' with "[HPC Hr1 Hr3 Hi]"); try iFrame; try solve_pure.
-    { admit. }
     iNext. iIntros "[(HPC & Hr3 & Hr1 & Hi & [%lmmio Hlmmio]) | (HPC & Hr3 & Hr1 & Hi)]".
     2: {
       (* Success false *)
@@ -327,23 +479,31 @@ Section SensorEnclaveProofs.
 
     (* "Initialize" the sensor. *)
     destruct (withinBounds mmio_b mmio_e mmio_a) eqn:Hmmiobounds.
-    2: { (* Store fail *) admit. }
+    2: {
+      (* Failure. Cursor out of bounds. *)
+      wp_instr. iInstr_lookup "Hts_code" as "Hi" "Hts_code".
+      iApply (wp_store_fail_z with "[$HPC $Hi $Hr1]");
+        try solve_pure; auto.
+      iIntros "!> _".
+      wp_pure. wp_end; by iIntros (?).
+    }
 
     iAssert ((∃ lw_a, (mmio_a, (mmio_v + 1)%nat) ↦ₐ lw_a)%I)
       with "[Hlmmio]" as "[%lw_a Hmmio_a]".
-    { pose proof (withinBounds_in_seq_1 _ _ _ Hmmiobounds) as Hlookup.
-      apply elem_of_list_lookup in Hlookup.
-      destruct Hlookup as [i Hlookup].
-      assert (exists lw_a, lmmio !! i = Some lw_a) as [lw_a Hlookup2] by admit.
-      iExists lw_a.
-      iDestruct (big_sepL2_lookup_acc with "Hlmmio") as "[Hmmio_a _]"; eauto.
-      now rewrite list_lookup_fmap Hlookup.
+    {
+      pose proof (withinBounds_in_seq_1 _ _ _ Hmmiobounds) as Hlookup.
+      pose proof (elem_of_list_fmap_1 (λ a : Addr, (a, (mmio_v + 1)%nat)) _ _ Hlookup)
+                 as Hlookup2.
+      apply elem_of_list_lookup in Hlookup2.
+      destruct Hlookup2 as [i Hlookup2].
+      by iDestruct (big_sepL2_extract_l' _ _ _ _ _ Hlookup2 with "Hlmmio")
+        as "[_ ?]".
     }
     iInstr "Hts_code". (* Store r_t1 42 *)
     clear lw_a.
 
     (* Get the data capability *)
-    iInstr "Hts_code". (* Lea r_t2 (begin - init) *)
+    iInstr "Hts_code". (* Lea r_t2 (begin - fail) *)
     transitivity (Some pc_b); [rewrite /sensor_fail_off; subst cf_b; solve_addr|easy].
     iInstr "Hts_code". (* Load r_t3 r_t2 *)
     easy.
@@ -356,11 +516,16 @@ Section SensorEnclaveProofs.
     transitivity (Some (data_b ^+ 1)%a); solve_addr.
 
     (* Store mmio capability. *)
-    iMod (one_shot_update with "Hts_data") as "[#Htoken Hts_data]"; try solve_addr.
-    iDestruct "Hts_data" as "[%Heq|[%lw Hts_mmio]]".
-    { admit. }
+    iMod (sensor_one_shot_update with "Hts_data") as "[#Htoken Hts_data]"; try solve_addr.
+    iDestruct "Hts_data" as "[%Hdatabounds1|(%Hdatabounds1 & %lw & Hts_mmio)]".
+    { (* Data section too small *)
+      wp_instr. iInstr_lookup "Hts_code" as "Hi" "Hts_code".
+      iApply (wp_store_fail_reg with "[$HPC $Hi $Hr3 $Hr1]");
+        try solve_pure; auto.
+      iIntros "!> _".
+      wp_pure. wp_end; by iIntros (?).
+    }
     iInstr "Hts_code". (* Store r_t3 r_t1 *)
-    admit. (* TODO: check for bounds in code *)
     clear lw.
 
     (* Get the seal/unseal master capability and switch to signing.  *)
@@ -372,10 +537,10 @@ Section SensorEnclaveProofs.
     { transitivity (Some (ot ^+1)%ot); solve_addr. }
 
     (* Construct read_sensor entry point. *)
-    iInstr "Hts_code". (* Lea r_t1 (read - fail) *)
-    { transitivity (Some (pc_b ^+ sensor_read_off))%a; [|easy].
-      rewrite /sensor_read_off. solve_addr. }
-    iInstr "Hts_code". (* Restrict r_t1 Eperm *)
+    iInstr "Hts_code". (* Lea r_t1 (read - begin) *)
+    { transitivity (Some (cf_b ^+ sensor_read_off))%a; [|easy].
+      rewrite /sensor_read_off. subst cf_b. solve_addr. }
+    iInstr "Hts_code". (* Restrict r_t2 Eperm *)
     { by rewrite decode_encode_perm_inv. }
     rewrite decode_encode_perm_inv.
 
@@ -407,33 +572,29 @@ Section SensorEnclaveProofs.
 
     set (lsealed_entry_read_cap := LSealedCap _ _ _ _ _ _).
     iAssert (interp lsealed_entry_read_cap) as "Hinterp_sealed_entry_read_cap".
-    {
-      iEval (rewrite /= fixpoint_interp1_eq /= /interp_sb).
-      iExists sealed_sensor; iFrame "%#".
-      iSplit.
-      { iPureIntro; intro; apply sealed_sensor_persistent. }
-      { iNext. do 4 iExists _. iSplit; [easy|]. iIntros (ret φ).
-        iApply (sensor_enclave_read_sensor_correct with "[$Henclave_inv $Hts_inv]");
-          subst cf_b cf_e pc_b pc_e; solve_addr.
-      }
-    }
+    { iEval (rewrite /= fixpoint_interp1_eq /= /interp_sb).
+      iExists sealed_sensor; iFrame "%#". iSplit.
+      - iPureIntro; intro; apply sealed_sensor_persistent.
+      - iNext. do 7 iExists _.
+        iSplit; first done.
+        iSplit; done. }
     iAssert (
         interp (LSealRange (false, true) (ot ^+ 1)%f (ot ^+ 2)%f (ot ^+ 1)%f)
       ) as "Hinterp_sealr_ot".
-    {
-      iEval (rewrite /= fixpoint_interp1_eq /= /safe_to_unseal).
-      iSplit ; first done.
+    { iEval (rewrite /= fixpoint_interp1_eq /= /safe_to_unseal).
+      iSplit; first done.
       rewrite finz_seq_between_singleton ; last solve_finz.
-      iSplit ; last done.
-      iSplit ; last done.
+      iSplit; last done.
+      iSplit; last done.
       iExists sealed_sensor_ne; iFrame "#".
       iNext ; iModIntro; iIntros (lw) "Hlw".
-      by iApply sealed_sensor_interp.
+      by iApply (sealed_sensor_interp with "[$Henclave_contract $Henclave_inv]").
     }
 
     (* Close the opened invariant *)
-    iMod ("Hclose" with "[$Hna $Hts_code $Hts_addr $Hts_keys Htoken Hts_mmio]") as "Hna".
-    iNext. iExists γ. iRight. iFrame "Htoken". do 4 iExists _. by iFrame.
+    iMod ("Hclose" with "[$Hna $Hts_code $Hts_addr $Hts_keys Htoken Hts_mmio Hmmio_a]") as "Hna".
+    iNext. iRight. iFrame "Htoken".
+    iSplit; [easy|]. do 4 iExists _. by iFrame "Hts_mmio Hmmio_a".
 
     (* Wrap up the registers *)
     iDestruct (big_sepM_insert _ _ r_t0 with "[$Hrmap $Hr0]") as "Hrmap".
@@ -479,6 +640,6 @@ Section SensorEnclaveProofs.
     }
 
     iApply ("Hjmp" with "[]") ; eauto ; iFrame.
-  Admitted.
+  Qed.
 
 End SensorEnclaveProofs.
